specs/Spec.Lib.IntVec.fst
@@ -1,90 +1,46 @@
 module Spec.Lib.IntVec
 
-open FStar.Seq
 open FStar.Mul
-
+open Spec.Lib.IntSeq
 module Ints = Spec.Lib.IntTypes
 
-type intvec (vt:vectype) = 
-  s:seq (Ints.uint_t vt.it){length s = vt.len}
-
-val seq_map_ghost:
-  #a:Type -> #b:Type ->
-  f:(a -> GTot b) ->
-  s:Seq.seq a ->
-  GTot (s':Seq.seq b{Seq.length s = Seq.length s' /\
-    (forall (i:nat). {:pattern (Seq.index s' i)} i < Seq.length s' ==> Seq.index s' i == f (Seq.index s i))})
-    (decreases (Seq.length s))
-let rec seq_map_ghost #a #b f s =
-  if Seq.length s = 0 then
-    Seq.createEmpty
-  else
-    let s' = Seq.cons (f (Seq.head s)) (seq_map_ghost f (Seq.tail s)) in
-    s'
-
-val seq_map:
-  #a:Type -> #b:Type ->
-  f:(a -> Tot b) ->
-  s:Seq.seq a ->
-  Tot (s':Seq.seq b{Seq.length s = Seq.length s' /\
-    (forall (i:nat). {:pattern (Seq.index s' i)} i < Seq.length s' ==> Seq.index s' i == f (Seq.index s i))})
-    (decreases (Seq.length s))
-let rec seq_map #a #b f s =
-  if Seq.length s = 0 then
-    Seq.createEmpty
-  else
-    let s' = Seq.cons (f (Seq.head s)) (seq_map f (Seq.tail s)) in
-    s'
-
-val seq_map2:
-  #a:Type -> #b:Type -> #c:Type ->
-  f:(a -> b -> Tot c) ->
-  s:Seq.seq a -> s':Seq.seq b{Seq.length s = Seq.length s'} ->
-  Tot (s'':Seq.seq c{Seq.length s = Seq.length s'' /\
-    (forall (i:nat). {:pattern (Seq.index s'' i)} i < Seq.length s'' ==> Seq.index s'' i == f (Seq.index s i) (Seq.index s' i))})
-    (decreases (Seq.length s))
-let rec seq_map2 #a #b #c f s s' =
-  if Seq.length s = 0 then Seq.createEmpty
-  else
-    let s'' = Seq.cons (f (Seq.head s) (Seq.head s')) (seq_map2 f (Seq.tail s) (Seq.tail s')) in
-    s''
-
+type intvec (vt:vectype) = lseq (Ints.uint_t vt.it) vt.len
 
 let intvec_v #vt v =
-  seq_map_ghost Ints.uint_v v
+  ghost_map Ints.uint_v v
 
 let vec_add #vt (v1:intvec vt) (v2:intvec vt) : intvec vt = 
-seq_map2 (Ints.add_mod #vt.it) v1 v2
+map2 (Ints.add_mod #vt.it) v1 v2
 
 let vec_sub #vt (v1:intvec vt) (v2:intvec vt) : intvec vt = 
-seq_map2 (Ints.sub_mod #vt.it) v1 v2
+map2 (Ints.sub_mod #vt.it) v1 v2
 
 let vec_mul #vt (v1:intvec vt) (v2:intvec vt): intvec vt = 
-seq_map2 (Ints.mul_mod #vt.it) v1 v2
+map2 (Ints.mul_mod #vt.it) v1 v2
 
 let vec_xor #vt (v1:intvec vt) (v2:intvec vt) : intvec vt = 
-seq_map2 (Ints.logxor #vt.it) v1 v2
+map2 (Ints.logxor #vt.it) v1 v2
 
 let vec_and #vt (v1:intvec vt) (v2:intvec vt) : intvec vt = 
-seq_map2 (Ints.logand #vt.it) v1 v2
+map2 (Ints.logand #vt.it) v1 v2
 
 let vec_or #vt (v1:intvec vt) (v2:intvec vt) : intvec vt = 
-seq_map2 (Ints.logor #vt.it) v1 v2
+map2 (Ints.logor #vt.it) v1 v2
 
 let vec_not #vt (v1:intvec vt) : intvec vt = 
-seq_map (Ints.lognot #vt.it) v1 
+map (Ints.lognot #vt.it) v1 
 
 let vec_shift_right #vt v1 s = 
-seq_map (fun x -> Ints.shift_right x s) v1 
+map (fun x -> Ints.shift_right x s) v1 
 
 let vec_shift_left #vt v1 s =
-seq_map (fun x -> Ints.shift_left #vt.it x s) v1 
+map (fun x -> Ints.shift_left #vt.it x s) v1 
 
 let vec_rotate_right #vt v1 s = 
-seq_map (fun x -> Ints.rotate_right  #vt.it x s) v1 
+map (fun x -> Ints.rotate_right  #vt.it x s) v1 
 
 let vec_rotate_left #vt v1 s = 
-seq_map (fun x -> Ints.rotate_left #vt.it x s) v1 
+map (fun x -> Ints.rotate_left #vt.it x s) v1 
 
 let op_Plus_Bar = vec_add
 let op_Subtraction_Bar = vec_sub
@@ -99,17 +55,20 @@ let op_Greater_Greater_Greater_Bar = vec_rotate_right
 let op_Less_Less_Less_Bar = vec_rotate_left
 
 let vec_load vt i = 
-  Seq.create vt.len i
+  create vt.len i
 
 let u32x4 i1 i2 i3 i4 = 
-  Seq.createL [i1;i2;i3;i4]
+  createL [i1;i2;i3;i4]
 
 let u32x8 i1 i2 i3 i4 i5 i6 i7 i8 = 
-  Seq.createL [i1;i2;i3;i4;i5;i6;i7;i8]
+  let l = [i1;i2;i3;i4;i5;i6;i7;i8] in
+  assert_norm (List.Tot.length l = 8);
+  createL l
 
 let u64x4 i1 i2 i3 i4 =
-  Seq.createL [i1;i2;i3;i4]
+  createL [i1;i2;i3;i4]
 
 let u64x2 i1 i2 = 
-  Seq.createL [i1;i2]
+  createL [i1;i2]
 
+    
